steel/Learn.Steel.ListP.Data.fst
@@ -1,0 +1,138 @@
+module Learn.Steel.ListP.Data
+
+module L   = FStar.List.Pure
+module US  = Learn.Steel.Util
+module T   = FStar.Tactics
+module Mem = Steel.Memory
+open Steel.Effect.Common
+open Steel.Reference
+
+open Learn.Steel.ListP.Param
+
+
+let mlist_cons_sel (p : list_param) (entry : ref p.r) (len' : nat) (exit : ref p.r)
+                   (sels : (c : t_of (p.cell entry).vp
+                              & mlist_sel_t p ((p.cell entry).get_next c) len' exit))
+  : GTot (mlist_sel_t p entry (len'+1) exit)
+  = let (|c, rs|) = sels in (|entry, (p.cell entry).get_data c|) :: rs
+
+let rec mlist0 (p : list_param) (entry : ref p.r) (len : nat) (exit : ref p.r)
+  : Pure vprop (requires True) (ensures fun v -> t_of v == mlist_sel_t p entry len exit)
+               (decreases %[len; 0])
+  =
+    if len = 0
+    then vrewrite (US.pure (entry == exit)) #(mlist_sel_t p entry len exit) (fun _ -> [])
+    else vrewrite ((p.cell entry).vp `vdep` mlist_cons_vp p entry (len-1) exit)
+                  (mlist_cons_sel p entry (len-1) exit)
+
+and mlist_cons_vp (p : list_param) (entry : ref p.r) (len' : nat) (exit : ref p.r) (c : t_of (p.cell entry).vp)
+  : Pure vprop (requires True) (ensures fun v -> t_of v == mlist_sel_t p ((p.cell entry).get_next c) len' exit)
+               (decreases %[len'; 1])
+  = mlist0 p ((p.cell entry).get_next c) len' exit
+
+
+
+let mlist_def (p : list_param) (entry : ref p.r) (len : nat) (exit : ref p.r)
+  : squash (mlist0 p entry len exit ==
+           (if len = 0
+            then vrewrite (US.pure (entry == exit)) #(mlist_sel_t p entry len exit) (fun _ -> [])
+            else vrewrite ((p.cell entry).vp `vdep` mlist_cons_vp p entry (len-1) exit)
+                          (mlist_cons_sel p entry (len-1) exit)))
+  = _ by T.(compute (); trefl ())
+
+let mlist_case_O (p : list_param) (entry : ref p.r) (exit : ref p.r)
+  : Lemma (mlist0 p entry 0 exit ==
+           vrewrite (US.pure (entry == exit)) #(mlist_sel_t p entry 0 exit) (fun _ -> []))
+  = mlist_def p entry 0 exit
+
+let mlist_case_S (p : list_param) (entry : ref p.r) (len : nat) (exit : ref p.r)
+  : Lemma (mlist0 p entry (len+1) exit ==
+           vrewrite ((p.cell entry).vp `vdep` mlist_cons_vp p entry len exit)
+                    (mlist_cons_sel p entry len exit))
+  = mlist_def p entry (len+1) exit
+
+let mlist_sel_case_S (p : list_param) (r0 : ref p.r) (len : nat) (exit : ref p.r) (m : Mem.mem)
+  : Lemma (requires Mem.interp (hp_of (mlist0 p r0 (len+1) exit)) m)
+          (ensures  Mem.interp (hp_of (p.cell r0).vp) m /\
+                   (let c = sel_of (p.cell r0).vp m in
+                    Mem.interp (hp_of (mlist_cons_vp p r0 len exit c)) m /\
+                    sel_of (mlist0 p r0 (len+1) exit) m ==
+                      mlist_cons_sel p r0 len exit (|c, sel_of (mlist_cons_vp p r0 len exit c) m|)))
+  =
+    mlist_case_S p r0 len exit;
+    interp_vdep_hp (p.cell r0).vp (mlist_cons_vp p r0 len exit) m;
+    calc (==) {
+      sel_of (mlist0 p r0 (len+1) exit) m;
+    == {}
+      vrewrite_sel ((p.cell r0).vp `vdep` mlist_cons_vp p r0 len exit)
+                   (mlist_cons_sel p r0 len exit) m;
+    == { vrewrite_sel_eq ((p.cell r0).vp `vdep` mlist_cons_vp p r0 len exit)
+                         (mlist_cons_sel p r0 len exit) m }
+       mlist_cons_sel p r0 len exit
+         (let (|c, rs|) =
+           ((sel_of ((p.cell r0).vp `vdep` mlist_cons_vp p r0 len exit) m)
+            <: vdep_t (p.cell r0).vp (mlist_cons_vp p r0 len exit))
+          in (|c, rs|));
+    == { vdep_sel_eq (p.cell r0).vp (mlist_cons_vp p r0 len exit) m }
+     (let c = sel_of (p.cell r0).vp m in
+      mlist_cons_sel p r0 len exit
+         (|c, sel_of (mlist_cons_vp p r0 len exit c) m|));
+    }
+
+(* expand the vprop *)
+
+let mlist_sl (p : list_param) entry len exit =
+  let VUnit r = mlist0 p entry len exit in r.hp
+
+let mlist_sel (p : list_param) (entry : ref p.r) (len : nat) (exit : ref p.r) =
+  let VUnit r = mlist0 p entry len exit in r.sel
+
+let mlist_eq0 (p : list_param) (entry : ref p.r) (len : nat) (exit : ref p.r)
+  : Lemma (mlist p entry len exit == mlist0 p entry len exit)
+          [SMTPat (mlist p entry len exit)]
+  = let VUnit _ = mlist0 p entry len exit in ()
+
+(* intro/elim lemmas *)
+
+let intro_mlist_nil_lem (p : list_param) (r0 : ref p.r) (m : Mem.mem)
+  : Lemma (ensures Mem.interp (hp_of (mlist0 p r0 0 r0)) m /\
+                   sel_of (mlist0 p r0 0 r0) m == [])
+  =
+    mlist_case_O p r0 r0;
+    US.intro_pure_lem (r0 == r0) m
+
+let elim_mlist_nil_lem (p : list_param) (r0 r1 : ref p.r) (m : Mem.mem)
+  : Lemma (requires Mem.interp (hp_of (mlist0 p r0 0 r1)) m)
+          (ensures  r0 == r1)
+  =
+    mlist_case_O p r0 r1;
+    US.elim_pure_lem (r0 == r1) m
+
+let intro_mlist_cons_lem (p : list_param) (r0 r1 : ref p.r) (len : nat) (exit : ref p.r) (m : Mem.mem)
+  : Lemma (requires Mem.interp (hp_of ((p.cell r0).vp `star` mlist0 p r1 len exit)) m /\
+                    (p.cell r0).get_next (sel_of (p.cell r0).vp m) == r1)
+          (ensures  Mem.interp (hp_of (mlist0 p r0 (len+1) exit)) m /\
+                    sel_of (mlist0 p r0 (len+1) exit) m ==
+                      (|r0, (p.cell r0).get_data (sel_of (p.cell r0).vp m)|)
+                      :: (sel_of (mlist0 p r1 len exit) m <: mlist_sel_t p r1 len exit))
+  =
+    mlist_case_S p r0 len exit;
+    interp_vdep_hp (p.cell r0).vp (mlist_cons_vp p r0 len exit) m;
+    mlist_sel_case_S p r0 len exit m
+
+let elim_mlist_cons_lem (p : list_param) (r0 : ref p.r)
+                        (hd : cell_t p) (tl : list (cell_t p))
+                        (len : nat) (exit : ref p.r) (m: Mem.mem)
+  : Lemma (requires Mem.interp (hp_of (mlist0 p r0 (len + 1) exit)) m /\
+                    (sel_of (mlist0 p r0 (len + 1) exit) m
+                      <: mlist_sel_t p r0 (len+1) exit) == hd :: tl)
+          (ensures (let r1 = sg_entry tl exit in
+                    Mem.interp (hp_of ((p.cell r0).vp `star` mlist p r1 len exit)) m /\
+                   (let c0 = sel_of (p.cell r0).vp m in
+                    (p.cell r0).get_next c0 == r1 /\
+                    (p.cell r0).get_data c0 == hd._2 /\
+                    sel_of (mlist0 p r1 len exit) m == tl)))
+  =
+    mlist_case_S p r0 len exit;
+    interp_vdep_hp (p.cell r0).vp (mlist_cons_vp p r0 len exit) m;
+    mlist_sel_case_S p r0 len exit m
