steel/Learn.Steel.ListP.Data.fsti
@@ -1,0 +1,69 @@
+module Learn.Steel.ListP.Data
+
+module L   = FStar.List.Pure
+module Mem = Steel.Memory
+open Steel.Effect.Common
+open Steel.Reference
+
+open Learn.Steel.ListP.Param
+
+let sg_entry (#r : Type) (#a : r -> Type) (l : list (x:r & a x)) (exit : r) : r =
+  match l with
+  | [] -> exit
+  | hd :: _ -> hd._1
+
+type mlist_sel_t (p : list_param) (entry : ref p.r) (len : nat) (exit : ref p.r) : Type =
+  l : list (cell_t p) {len = L.length l /\ entry == sg_entry l exit}
+
+val mlist_sl (p : list_param u#0) (entry : ref p.r) (len : nat) (exit : ref p.r)
+  : Mem.slprop u#1
+
+val mlist_sel (p : list_param) (entry : ref p.r) (len : nat) (exit : ref p.r)
+  : selector (mlist_sel_t p entry len exit) (mlist_sl p entry len exit)
+
+[@@__steel_reduce__]
+let mlist' (p : list_param) (entry : ref p.r) ([@@@smt_fallback] len : nat) (exit : ref p.r) : vprop' =
+  {
+    hp  = mlist_sl    p entry len exit;
+    t   = mlist_sel_t p entry len exit;
+    sel = mlist_sel   p entry len exit
+  }
+unfold let mlist (p : list_param) (entry : ref p.r) ([@@@smt_fallback] len : nat) (exit : ref p.r) : vprop =
+  VUnit (mlist' p entry len exit)
+
+[@@ __steel_reduce__]
+let sel_list (#q:vprop) (p : list_param) (entry : ref p.r) (len : nat) (exit : ref p.r)
+  (h:rmem q{FStar.Tactics.with_tactic selector_tactic (can_be_split q (mlist p entry len exit) /\ True)})
+  : GTot (mlist_sel_t p entry len exit)
+  = h (mlist p entry len exit)
+
+(* intro/elim lemmas *)
+
+val intro_mlist_nil_lem (p : list_param) (r0 : ref p.r) (m : Mem.mem)
+  : Lemma (ensures Mem.interp (hp_of (mlist p r0 0 r0)) m /\
+                   (sel_of (mlist p r0 0 r0) m <: mlist_sel_t p r0 0 r0) == [])
+
+val elim_mlist_nil_lem (p : list_param) (r0 r1 : ref p.r) (m : Mem.mem)
+  : Lemma (requires Mem.interp (hp_of (mlist p r0 0 r1)) m)
+          (ensures  r0 == r1)
+
+val intro_mlist_cons_lem (p : list_param) (r0 r1 : ref p.r) (len : nat) (exit : ref p.r) (m : Mem.mem)
+  : Lemma (requires Mem.interp (hp_of ((p.cell r0).vp `star` mlist p r1 len exit)) m /\
+                    (p.cell r0).get_next (sel_of (p.cell r0).vp m) == r1)
+          (ensures  Mem.interp (hp_of (mlist p r0 (len+1) exit)) m /\
+                    sel_of (mlist p r0 (len+1) exit) m ==
+                      (|r0, (p.cell r0).get_data (sel_of (p.cell r0).vp m)|)
+                      :: (sel_of (mlist p r1 len exit) m <: mlist_sel_t p r1 len exit))
+
+val elim_mlist_cons_lem (p : list_param) (r0 : ref p.r)
+                        (hd : cell_t p) (tl : list (cell_t p))
+                        (len : nat) (exit : ref p.r) (m: Mem.mem)
+  : Lemma (requires Mem.interp (hp_of (mlist p r0 (len + 1) exit)) m /\
+                    (sel_of (mlist p r0 (len + 1) exit) m
+                      <: mlist_sel_t p r0 (len+1) exit) == hd :: tl)
+          (ensures (let r1 = sg_entry tl exit in
+                    Mem.interp (hp_of ((p.cell r0).vp `star` mlist p r1 len exit)) m /\
+                   (let c0 = sel_of (p.cell r0).vp m in
+                    (p.cell r0).get_next c0 == r1 /\
+                    (p.cell r0).get_data c0 == hd._2 /\
+                    sel_of (mlist p r1 len exit) m == tl)))
