steel/Learn.Steel.ListP.Derived.fst
@@ -1,0 +1,27 @@
+module Learn.Steel.ListP.Derived
+
+let v (p : list_param) (entry : ref p.r) (len : nat)
+  = mlist p entry len null
+
+let f (p : list_param) (entry : ref p.r) (len : nat) (l : t_of (v p entry len)) : mlistN_sel_t p entry
+  = l
+
+let mlistN_sl (p : list_param) (entry : ref p.r) =
+  US.vexists_sl (v p entry)
+
+let mlistN_indep (p : list_param) (entry : ref p.r)
+  : Lemma (ensures US.vexists_indep (v p entry) (f p entry))
+  = US.vexists_indepI_unique (v p entry) (mlistN_length_unique p entry)
+
+let mlistN_sel (p : list_param) (entry : ref p.r) =
+  mlistN_indep p entry;
+  US.vexists_sel (v p entry) (f p entry)
+
+let intro_mlistN #opened (p : list_param) entry len =
+  mlistN_indep p entry;
+  US.intro_vexists len (v p entry) (f p entry)
+
+let elim_mlistN #opened (p : list_param) entry
+  =
+    mlistN_indep p entry;
+    US.witness_vexists (v p entry) (f p entry)
