steel/Learn.Steel.ListP.Param.fst
@@ -1,0 +1,64 @@
+module Learn.Steel.ListP.Param
+
+module US  = Learn.Steel.Util
+module Mem = Steel.Memory
+open Steel.Effect.Common
+open Steel.Effect
+open Steel.Reference
+
+
+noeq inline_for_extraction noextract
+type list_param_r' (r : Type) = {
+  vp        : vprop;
+  data_t    : Type;
+  get_next  : normal (t_of vp) -> GTot (ref r);
+  set_next  : normal (t_of vp) -> (nxt:ref r) -> GTot (c:normal (t_of vp) {get_next c == nxt});
+  get_data  : normal (t_of vp) -> GTot data_t;
+
+  read_next  : unit -> Steel (ref r) vp (fun _ -> vp) (requires fun _ -> True)
+                      (ensures fun h0 x h1 -> frame_equalities vp h0 h1 /\ x == get_next (h0 vp));
+  write_next : (x : ref r) -> Steel unit vp (fun _ -> vp) (requires fun _ -> True)
+                      (ensures fun h0 () h1 -> h1 vp == set_next (h0 vp) x)
+}
+
+inline_for_extraction noextract
+type list_param_r (r : Type) = p:list_param_r' r {
+  (forall (s : normal (t_of p.vp)) (x0 x1 : ref r) . {:pattern (p.set_next (p.set_next s x0) x1)}
+      p.set_next (p.set_next s x0) x1 == p.set_next s x1) /\
+  (forall (s : normal (t_of p.vp)) . {:pattern (p.set_next s (p.get_next s))}
+      p.set_next s (p.get_next s) == s) /\
+  (forall (s : normal (t_of p.vp)) (x:ref r) . {:pattern (p.get_data (p.set_next s x))}
+     p.get_data (p.set_next s x) == p.get_data s)
+}
+
+noeq inline_for_extraction noextract
+type list_param = {
+  r      : Type;
+  cell   : ref r -> list_param_r r;
+  nnull  : (x : ref r) -> (m : Mem.mem) ->
+           Lemma (requires Mem.interp (hp_of (cell x).vp) m)
+                 (ensures  is_null x == false)
+}
+
+let cell_t (p : list_param) : Type = x:ref p.r & (p.cell x).data_t
+
+inline_for_extraction noextract
+let aptr_next (p : list_param) (x : ref p.r) : US.aptr (ref p.r) = {
+  vp      = (p.cell x).vp;
+  of_sel  = (p.cell x).get_next;
+  set_sel = (p.cell x).set_next;
+  read    = (p.cell x).read_next;
+  write   = (p.cell x).write_next
+}
+
+[@@ __steel_reduce__]
+let g_next (#q:vprop) (p:list_param) (x:ref p.r)
+  (h:rmem q{FStar.Tactics.with_tactic selector_tactic (can_be_split q (p.cell x).vp /\ True)})
+  : GTot (ref p.r)
+  = (p.cell x).get_next (h (p.cell x).vp)
+
+[@@ __steel_reduce__]
+let g_data (#q:vprop) (p:list_param) (x:ref p.r)
+  (h:rmem q{FStar.Tactics.with_tactic selector_tactic (can_be_split q (p.cell x).vp /\ True)})
+  : GTot ((p.cell x).data_t)
+  = (p.cell x).get_data (h (p.cell x).vp)
